Working towards catch-up and recovery.
Added a crash and recovery action.
Added an explicit log for the recovery.

Isabelle2/AbstractMultiPaxosR1.thy
@@ -2,19 +2,20 @@ theory AbstractMultiPaxosR1
 imports  IOA BallotArrays DistributedSafeAt Paxos_Sig
 begin
 
-record ('v,'a,'l) ampr1_state =
+record ('v,'a) ampr1_state =
   propCmd :: "'v set"
   ballot :: "'a \<Rightarrow> bal"
   vote :: "'a \<Rightarrow> inst \<Rightarrow> bal \<rightharpoonup> 'v"
   suggestion :: "inst \<Rightarrow> bal \<rightharpoonup> 'v"
+  twoas :: "inst \<Rightarrow> bal \<rightharpoonup> 'v"
+  -- {* suggestion is forgotten upon a crash, but the twoa messages stay in the network. *}
   onebs :: "'a \<Rightarrow> bal \<rightharpoonup> (inst \<Rightarrow> ('v\<times>bal) set)"
   inst_status :: "bal \<rightharpoonup> inst \<rightharpoonup> 'v"
   -- {* if @{term "inst_status s b = Some m"}, them @{term "m i = None"} means that 
   all values are safe, and @{term "m i = Some v"} means that only @{term v} is known safe. *}
   log :: "'a \<Rightarrow> inst \<Rightarrow> 'v option"
   -- {* The log is there to transfer it to replicas who need to catch up. *}
-  lowest_inst :: "'a \<Rightarrow> inst"
-  -- {* The lowest for which an acceptor has a log (grows because of garbage collection.*}
+  crashed :: "'a \<Rightarrow> bool"
 
 locale ampr1_ioa =
   fixes quorums::"'a set set" and leader :: "bal \<Rightarrow> 'a"
@@ -26,9 +27,9 @@ sublocale dsa:distributed_safe_at quorums ballot vote for ballot vote .
 definition start_s where
   -- {* The initial state *}
   "start_s \<equiv> \<lparr>propCmd = {}, ballot = (\<lambda> a . 0), vote = (\<lambda> a i . Map.empty), 
-    suggestion = \<lambda> i . Map.empty, onebs = \<lambda> a . Map.empty,
+    suggestion = \<lambda> i . Map.empty, twoas = \<lambda> i . Map.empty, onebs = \<lambda> a . Map.empty,
     inst_status = \<lambda> b . if b = 0 then Some Map.empty else None,
-    log = \<lambda> a . Map.empty, lowest_inst = \<lambda> a . 0\<rparr>"
+    log = \<lambda> a . Map.empty, crashed = \<lambda> a . False\<rparr>"
 
 definition start where "start \<equiv> {start_s}"
   
@@ -41,12 +42,14 @@ definition join_ballot where
   "join_ballot a b s s' \<equiv>
     let onebs' = \<lambda> i . dsa.acc_max (flip (vote s) i) a b
     in
-      b > (ballot s a)
+      crashed s a = False
+      \<and> b > (ballot s a)
       \<and> s' = s\<lparr>ballot := (ballot s)(a := b),
         onebs := (onebs s)(a := (onebs s a)(b \<mapsto> onebs'))\<rparr>"
   
 definition join_started_ballot where "join_started_ballot a b s s' \<equiv>
-  inst_status s b \<noteq> None 
+  crashed s a = False
+  \<and> inst_status s b \<noteq> None 
   \<and> ballot s a < b
   \<and> s' = s\<lparr>ballot := (ballot s)(a := b)\<rparr>"
   
@@ -62,39 +65,59 @@ definition acquire_leadership where
   -- {* Upon acquiring leadership, the leader makes suggestions in an
   arbitrary set of instances which have a unique safe value. *}
   "acquire_leadership a q s s' \<equiv> let b = ballot s a in
-    leader b = a
+    crashed s a = False
+    \<and> leader b = a
     \<and> q \<in> quorums
     \<and> joined s q b
     \<and> inst_status s b = None
     \<and> inst_status s' = (inst_status s)(b := Some (\<lambda> i . sugg s i b q))
     \<and> (\<forall> i . suggestion s' i = (suggestion s i)(b := sugg s i b q) 
       \<or> suggestion s' i = (suggestion s i))
-    \<and> propCmd s' = propCmd s \<and> ballot s' = ballot s \<and> vote s' = vote s \<and> onebs s' = onebs s"
-
+    \<and> (\<forall> i . twoas s' i = (twoas s i)(b := suggestion s' i b))
+    \<and> propCmd s' = propCmd s \<and> ballot s' = ballot s \<and> vote s' = vote s 
+    \<and> onebs s' = onebs s \<and> log s' = log s"
+  
 definition suggest where "suggest a i b v s s' \<equiv>
-          v \<in> propCmd s
-        \<and> ballot s a = b
-        \<and> suggestion s i b = None
-        \<and> (case inst_status s b of Some f \<Rightarrow> f i = None | _ \<Rightarrow> False)
-        \<and> s' = s\<lparr>suggestion := (suggestion s)(i := (suggestion s i)(b \<mapsto> v))\<rparr>"
-
+  crashed s a = False
+  \<and> v \<in> propCmd s
+  \<and> ballot s a = b
+  \<and> suggestion s i b = None
+  \<and> (case inst_status s b of Some f \<Rightarrow> f i = None | _ \<Rightarrow> False)
+  \<and> s' = s\<lparr>suggestion := (suggestion s)(i := (suggestion s i)(b \<mapsto> v)),
+    twoas := (twoas s)(i := (twoas s i)(b \<mapsto> v))\<rparr>"
+  
 definition do_vote where
   "do_vote a i v s s' \<equiv> let b = ballot s a in
-          vote s a i b = None
-        \<and> suggestion s i b = Some v
-        \<and> s' = s\<lparr>vote := (vote s)(a := (vote s a)(i := (vote s a i)(b := Some v))),
-            log := (log s)(a := (log s a)(i := Some v))\<rparr>"
+    crashed s a = False
+    \<and> vote s a i b = None
+    \<and> twoas s i b = Some v
+    \<and> s' = s\<lparr>vote := (vote s)(a := (vote s a)(i := (vote s a i)(b := Some v)))\<rparr>"
 
 definition chosen where
-  "chosen s i v \<equiv> ballot_array.chosen quorums (flip (vote s) i) v"
+  "chosen s i v \<equiv> dsa.chosen (flip (vote s) i) v"
 
 definition learn where
-  "learn i vs s s' \<equiv> s' = s \<and> (\<forall> j < length vs . chosen s (i+j) (vs!(j+1)))"
+  "learn a i v s s' \<equiv>
+    crashed s a = False
+    \<and> s' = s\<lparr>log := (log s)(a := (log s a)(i := Some v))\<rparr>
+    \<and> chosen s i v"
   
-definition re_join where 
-  "re_join a\<^sub>1 a\<^sub>2 s s' \<equiv> 
-    s' = s\<lparr>ballot := (ballot s)(a\<^sub>1 := ballot s a\<^sub>2),
-      lowest_inst := (lowest_inst s)(a\<^sub>1 := lowest_inst s a\<^sub>2)\<rparr>"
+definition crash where
+  "crash a s s' \<equiv> \<exists> su . 
+    (\<forall> i b . (leader b = a \<and> su i b = None) \<or> (leader b \<noteq> a \<and> su i b = suggestion s i b))
+    \<and> s' = s\<lparr>suggestion := su, crashed := (crashed s)(a := True)\<rparr>"
+  
+definition recover where
+  -- {* Download the log from a2. Models recovery after a crash; ballot is persistent.
+    We increment the ballot to make sure not to produce inconsistent suggestions if
+    the crashed acceptor was the leader. *}
+  "recover a1 a2 i vs s s' \<equiv> 
+    crashed s a1 = True
+    \<and> (\<forall> j . i \<le> j \<and> j < i+(length vs) \<longrightarrow> log s a2 j = Some (vs!(j-i+1)))
+    \<and> s' = s\<lparr>ballot := (ballot s)(a1 := (let b = ballot s a1 in
+        if leader b = a1 then Suc b else b)),
+      log := (log s)(a1 := (log s a2)),
+      crashed := (crashed s)(a1 := False)\<rparr>"
 
 fun trans_rel where
   "trans_rel r (Propose c) r' = propose c r r'"
@@ -103,19 +126,24 @@ fun trans_rel where
     \<or> (\<exists> a i v . do_vote a i v r r')
     \<or> (\<exists> a i b v . suggest a i b v r r')
     \<or> (\<exists> a q . acquire_leadership a q r r')
-    \<or> (\<exists> a b . join_started_ballot a b r r') )"
-| "trans_rel r (Learn i vs) r' = learn i vs r r'"
+    \<or> (\<exists> a b . join_started_ballot a b r r')
+    \<or> (\<exists> a . crash a r r') )"
+  | "trans_rel r (Learn a i vs) r' = (
+    (\<exists> v . learn a i v r r' \<and> vs = [v])
+    \<or> (\<exists> a\<^sub>1 a\<^sub>2 . recover a\<^sub>1 a\<^sub>2 i vs r r') )"
 
 lemma trans_cases:
   assumes "trans_rel r a r'"
   obtains 
   (propose) c where "propose c r r'"
-| (learn) i v where "learn i v r r'"
+| (learn) a i v where "learn a i v r r'"
 | (join_ballot) a b where "join_ballot a b r r'"
 | (do_vote) a i v where "do_vote a i v r r'"
 | (suggest) a i b v where "suggest a i b v r r'"
 | (acquire) a q where "acquire_leadership a q r r'"
 | (join_started) a b where "join_started_ballot a b r r'"
+| (recover) a\<^sub>1 a\<^sub>2 i vs where "recover a\<^sub>1 a\<^sub>2 i vs r r'"
+| (crash) a where "crash a r r'"
   using assms apply induct apply simp
   by (metis ampr1_ioa.trans_rel.simps(1) ampr1_ioa.trans_rel.simps(3) paxos_action.exhaust trans_rel.simps(2)) 
 
