Isabelle2/Paxos_Sig.thy
@@ -2,15 +2,16 @@ theory Paxos_Sig
 imports Main Utils IOA
 begin
 
-datatype 'v paxos_action =
+datatype ('a,'v) paxos_action =
   Propose 'v
-  | Learn inst 'v
+  | Learn 'a inst "'v list"
+    -- {* learn about a list of instances starting at the given instance. *}
   | Internal
 
 definition paxos_asig where
 "paxos_asig \<equiv>
   \<lparr> inputs = { Propose c | c . True},
-    outputs = { Learn i v | i v . True},
+    outputs = { Learn a i vs | a i vs . True},
     internals = {Internal} \<rparr>"
 
 end
